open import Cubical.Foundations.Prelude
open import Cubical.Data.Bool
open import Cubical.Data.Sigma
open import Cubical.Functions.Fixpoint
open import Cubical.Relation.Nullary.Base
open import Cubical.Data.Empty using (âŠ¥) renaming (rec to recEmpty)

module computability.rice where

variable
  â„“ : Level
  A : Type â„“

byAbsurdity : {Anything : Type â„“} â†’ âŠ¥ â†’ Anything
byAbsurdity x = recEmpty x

ğŸš = Bool

_==_ : ğŸš â†’ ğŸš â†’ ğŸš
true == true = true
false == false = true
a == b = false

not-eq-bool : (a b : ğŸš) â†’ (Â¬ a â‰¡ b) â†’ a == b â‰¡ false
not-eq-bool false true H = refl
not-eq-bool true false H = refl
not-eq-bool false false H = byAbsurdity (H refl)
not-eq-bool true true H = byAbsurdity (H refl)

eq-bool : (a b : ğŸš) â†’ a â‰¡ b â†’ a == b â‰¡ true
eq-bool false false H = refl
eq-bool false true H = H
eq-bool true false H = sym H
eq-bool true true H = H

module _ (fA : (e : A â†’ A) â†’ Fixpoint e) (f : A â†’ ğŸš) (x y : A) where
  g : A â†’ A
  g z = if f z == f y then x else y
  u : A
  u = fixpoint (fA g)

  guâ‰¡u : g u â‰¡ u
  guâ‰¡u = fixpointPath (fA g)

  rice : f x â‰¡ f y
  rice with f u â‰Ÿ f y
  ...| yes P = f x â‰¡âŸ¨ sym (congS f uâ‰¡x) âŸ©
               f u â‰¡âŸ¨ P âŸ©
               f y âˆ
    where
    uâ‰¡x : u â‰¡ x
    uâ‰¡x =
      u â‰¡âŸ¨ sym guâ‰¡u âŸ©
      g u â‰¡âŸ¨ refl âŸ©
      (if f u == f y then x else y) â‰¡âŸ¨ cong (Î» b â†’ if b then x else y) (eq-bool (f u) (f y) P) âŸ©
      (if true then x else y) â‰¡âŸ¨ refl âŸ©
      x âˆ
  ...| no P = f x â‰¡âŸ¨ sym (congS f uâ‰¡x) âŸ©
              f u â‰¡âŸ¨ l' âŸ©
              f y âˆ
    where
    noteq : f u == f y â‰¡ false
    noteq = not-eq-bool (f u) (f y) P
    l : u â‰¡ y
    l =
      u â‰¡âŸ¨ sym (fA g .snd) âŸ©
      g u â‰¡âŸ¨ refl âŸ©
      (if f u == f y then x else y) â‰¡âŸ¨ cong (Î» b â†’ if b then x else y) noteq âŸ©
      (if false then x else y) â‰¡âŸ¨ refl âŸ©
      y âˆ
    l' : f u â‰¡ f y
    l' = congS f l
    uâ‰¡x : u â‰¡ x
    uâ‰¡x =
      u â‰¡âŸ¨ sym guâ‰¡u âŸ©
      g u â‰¡âŸ¨ refl âŸ©
      (if f u == f y then x else y) â‰¡âŸ¨ cong (Î» b â†’ if b then x else y) (eq-bool (f u) (f y) l') âŸ©
      (if true then x else y) â‰¡âŸ¨ refl âŸ©
      x âˆ
